x86/RawAsmgen.v
@@ -1,0 +1,204 @@
+Require Import Smallstep.
+Require Import Machregs.
+Require Import Asm.
+Require Import Integers.
+Require Import List.
+Require Import ZArith.
+Require Import Memtype.
+Require Import Memory.
+Require Import Archi.
+Require Import Coqlib.
+Require Import AST.
+Require Import Globalenvs.
+Require Import Events.
+Require Import Values.
+Require Import Conventions1.
+
+Section WITHMEMORYMODEL.
+
+  Context `{memory_model_ops: Mem.MemoryModelOps}.
+
+  Existing Instance mem_accessors_default.
+
+  Context `{!ExternalCallsOps mem} `{!EnableBuiltins mem}.
+
+  Definition exec_instr {F V} (ge: Genv.t F V) f i rs m :=
+    match i with
+    | Pallocframe fi ofs_ra ofs_link =>
+      let sp := Val.offset_ptr (rs # RSP) (Ptrofs.repr (- (frame_size fi))) in
+      match Mem.storev Mptr m (Val.offset_ptr sp ofs_link) rs#RSP with
+      | None => Stuck
+      | Some m2 =>
+        match Mem.storev Mptr m2 (Val.offset_ptr sp ofs_ra) rs#RA with
+        | None => Stuck
+        | Some m3 => Next (nextinstr (rs #RAX <- (rs#RSP) #RSP <- sp)) m3
+        end
+      end
+    | Pfreeframe sz ofs_ra ofs_link =>
+      match Mem.loadv Mptr m (Val.offset_ptr rs#RSP ofs_ra) with
+      | None => Stuck
+      | Some ra =>
+        match Mem.loadv Mptr m (Val.offset_ptr rs#RSP ofs_link) with
+        | None => Stuck
+        | Some sp =>
+          match rs#RSP with
+          | Vptr stk ofs => Next (nextinstr (rs#RSP <- sp #RA <- ra)) m
+          | _ => Stuck
+          end
+        end
+      end
+    | _ => Asm.exec_instr ge f i rs m
+    end.
+
+  Inductive step (ge: Genv.t Asm.fundef unit) : state -> trace -> state -> Prop :=
+  | exec_step_internal:
+      forall b ofs f i rs m rs' m',
+        rs PC = Vptr b ofs ->
+        Genv.find_funct_ptr ge b = Some (Internal f) ->
+        find_instr (Ptrofs.unsigned ofs) (fn_code f) = Some i ->
+        exec_instr ge f i rs m = Next rs' m' ->
+        step ge (State rs m) E0 (State rs' m')
+  | exec_step_builtin:
+      forall b ofs f ef args res rs m vargs t vres rs' m',
+        rs PC = Vptr b ofs ->
+        Genv.find_funct_ptr ge b = Some (Internal f) ->
+        find_instr (Ptrofs.unsigned ofs) f.(fn_code) = Some (Pbuiltin ef args res) ->
+        eval_builtin_args ge rs (rs RSP) m args vargs ->
+        external_call ef ge vargs m t vres m' ->
+        forall BUILTIN_ENABLED: builtin_enabled ef,
+          rs' = nextinstr_nf
+                  (set_res res vres
+                           (undef_regs (map preg_of (destroyed_by_builtin ef)) rs)) ->
+          step ge (State rs m) t (State rs' m')
+  | exec_step_external:
+      forall b ef args res rs m t rs' m',
+        rs PC = Vptr b Ptrofs.zero ->
+        Genv.find_funct_ptr ge b = Some (External ef) ->
+        extcall_arguments rs m (ef_sig ef) args ->
+        forall (SP_TYPE: Val.has_type (rs RSP) Tptr)
+          (RA_TYPE: Val.has_type (rs RA) Tptr)
+          (SP_NOT_VUNDEF: rs RSP <> Vundef)
+          (RA_NOT_VUNDEF: rs RA <> Vundef), 
+          external_call ef ge args m t res m' ->
+          rs' = (set_pair (loc_external_result (ef_sig ef)) res (undef_regs (CR ZF :: CR CF :: CR PF :: CR SF :: CR OF :: nil) (undef_regs (map preg_of destroyed_at_call) rs))) #PC <- (rs RA) #RA <- Vundef ->
+          step ge (State rs m) t (State rs' m').
+
+  Variable prog: Asm.program.
+  Let ge := Genv.globalenv prog.
+
+  Inductive match_states: state -> state -> Prop := 
+  | match_states_intro:
+      forall j rs m rs' m' bnd
+        (MINJ: Mem.inject j m m')
+        (RINJ: forall r, Val.inject j (rs # r) (rs' # r))
+        (MPG: Separation.globalenv_preserved ge j bnd)
+      ,
+        match_states (State rs m) (State rs' m').
+
+  Axiom exec_instr_inject:
+    forall j m1 m2 rs1 rs2 f i rs1' m1',
+      Mem.inject j m1 m2 ->
+      (forall r, Val.inject j (rs1#r) (rs2#r)) ->
+      Asm.exec_instr ge f i rs1 m1 = Next rs1' m1' ->
+      exists j' rs2' m2',
+        Asm.exec_instr ge f i rs2 m2 = Next rs2' m2'
+        /\ Mem.inject j' m1' m2'
+        /\ (forall r, Val.inject j' (rs1'#r) (rs2'#r))
+        /\ inject_incr j j'.
+  (* should be proved already somewhere *)
+
+  Definition is_unchanged (i: instruction) :=
+    match i with
+      Pallocframe _ _ _ 
+    | Pfreeframe _ _ _ => false
+    | _ => true
+    end.
+
+  Variable bstack: block.
+  Variable id_stack: ident.
+  Hypothesis find_bstack: Genv.find_symbol ge id_stack = Some bstack. 
+
+  Lemma alloc_inject:
+    forall j m1 m2 rs1 rs2 f i rs1' m1',
+      Mem.inject j m1 m2 ->
+      (forall r, Val.inject j (rs1#r) (rs2#r)) ->
+      Mem.alloc m 0 (frame_size fi) = (m', b) ->
+      Mem.record_stack_blocks m' (inl (b, Some fi)) (frame_size fi) = Some m'' ->
+      rs2 # RSP = 
+      exists j',
+        j' b = 
+
+  Lemma exec_instr_inject':
+    forall j m1 m2 rs1 rs2 f i rs1' m1',
+      Mem.inject j m1 m2 ->
+      (forall r, Val.inject j (rs1#r) (rs2#r)) ->
+      Asm.exec_instr ge f i rs1 m1 = Next rs1' m1' ->
+      exists j' rs2' m2',
+        exec_instr ge f i rs2 m2 = Next rs2' m2'
+        /\ Mem.inject j' m1' m2'
+        /\ (forall r, Val.inject j' (rs1'#r) (rs2'#r))
+        /\ inject_incr j j'.
+  Proof.
+    intros. destruct (is_unchanged i) eqn:?.
+    edestruct exec_instr_inject; eauto.
+    destruct i; simpl in *; eauto; try congruence.
+    destruct i; simpl in *; try congruence.
+    -                           (* allocframe *)
+      repeat destr_in H1.
+      
+  Qed.
+
+  
+  
+  Theorem step_simulation:
+    forall S1 t S2, Asm.step ge S1 t S2 ->
+               forall S1' (MS: match_states S1 S1'),
+                 (exists S2', step ge S1' t S2' /\ match_states S2 S2').
+  Proof.
+    destruct 1; intros; inv MS.
+    -
+      generalize (RINJ PC); rewrite H. inversion 1; subst.
+      assert (j b = Some (b,0)) as JB.
+      {
+        destruct MPG.
+        apply DOMAIN.
+        eapply FUNCTIONS. eauto. 
+      }
+      rewrite JB in H7; inv H7. 
+      generalize (exec_instr_inject _ _ _ _ _ _ _ _ _ MINJ RINJ H2).
+      intros (j' & rs2' & m2' & EI & MINJ' & RINJ' & INCR).
+      destruct (is_unchanged i) eqn:?.
+      eexists; split.
+      eapply exec_step_internal; eauto.
+      rewrite Ptrofs.add_zero. eauto.
+      instantiate (1 := m2'). instantiate (1:= rs2').
+      rewrite <- EI. destruct i; simpl in *; try congruence.
+      econstructor; eauto.
+      admit.
+      destruct i; simpl in Heqb; try congruence.
+      + 
+        eexists; split.
+        eapply exec_step_internal; eauto.
+        rewrite Ptrofs.add_zero. eauto.
+        instantiate (1 := m2'). instantiate (1:= rs2').
+
+
+        simpl in EI.
+        eapply Ageneralize (Genv.find_funct_ptr_transf match_prog _ H0). intro FFP.
+      generalize (find_instr_transl _ _ _ H1); intro FINSTR.
+
+      assert (match i with
+                Pallocframe _ _ _
+              | Pfreeframe _ _ _ => False
+              | _ => True
+              end \/ (match i with
+                Pallocframe _ _ _
+              | Pfreeframe _ _ _ => True
+              | _ => False
+              end)) as DEC.
+      {
+        destruct i; simpl; auto.
+      }
+      destruct DEC.
+
+  Qed.
