Makefile
@@ -96,7 +96,9 @@ BACKEND=\
   Mach.v \
   EraseArgs.v \
   Bounds.v Stacklayout.v Stacking.v Stackingproof.v \
-  Asm.v Asmgen.v Asmgenproof0.v Asmgenproof1.v Asmgenproof.v
+  Asm.v Asmgen.v Asmgenproof0.v Asmgenproof1.v Asmgenproof.v \
+	RawAsmgen.v
+
 #  Tailcall.v Tailcallproof.v \
 #  Inlining.v Inliningspec.v Inliningproof.v \
  
